src/MVector.thy
@@ -11,13 +11,13 @@ primrec size_of_mvector where
   "size_of_mvector (MVector _ s) = s"
 
 definition alloc :: "nat \<Rightarrow> heap \<Rightarrow> 'a::heap mvector \<times> heap" where
-  "alloc n h = (let l = lim h; r = MVector l n in (r, h \<lparr> lim := lim h + Addr n \<rparr>))"
+  "alloc n h = (let l = lim h; r = MVector l n in (r, h \<lparr> lim := lim h + n \<rparr>))"
 
 definition get_at :: "heap \<Rightarrow> 'a::heap mvector \<Rightarrow> nat \<Rightarrow> 'a" where
-  "get_at h v i = from_nat (memory h (addr_of_mvector v + Addr i))"
+  "get_at h v i = from_nat (memory h (addr_of_mvector v + i))"
 
 definition set_at :: "'a::heap mvector \<Rightarrow> nat \<Rightarrow> 'a \<Rightarrow> heap \<Rightarrow> heap" where
-  "set_at r j v h = h \<lparr> memory := (\<lambda>i. if i = addr_of_mvector r + Addr j then to_nat v else memory h i) \<rparr>"
+  "set_at r j v h = h \<lparr> memory := (\<lambda>i. if i = addr_of_mvector r + j then to_nat v else memory h i) \<rparr>"
 
 definition new :: "nat \<Rightarrow> 'a::heap mvector io" where
   "new n = IO (alloc n)"
@@ -43,19 +43,23 @@ definition swap :: "'a::heap mvector \<Rightarrow> nat \<Rightarrow> nat \<Right
 lemma get_set_eq [simp]: "get_at (set_at r i x h) r i = x"
   by (simp add: get_at_def set_at_def)
 
+lemma get_set_neq: "i \<noteq> j \<Longrightarrow> get_at (set_at r i x h) r j = get_at h r j"
+  apply (auto simp add: get_at_def set_at_def)
+  done
+
 lemma set_same [simp]: "set_at r j x (set_at r j y h) = set_at r j x h"
   apply (simp add: set_at_def)
 proof-
   have "\<And>P x y. P x \<Longrightarrow> (\<And>y. x \<noteq> y \<Longrightarrow> P y) \<Longrightarrow> (\<And>z. P z)"
     by metis
-  hence "\<And>f g. f (addr_of_mvector r + Addr j) = g (addr_of_mvector r + Addr j)
-    \<Longrightarrow> (\<And>x. x \<noteq> addr_of_mvector r + Addr j \<Longrightarrow> f x = g x) \<Longrightarrow> (\<And>z. f z = g z)"
+  hence "\<And>f g. f (addr_of_mvector r + j) = g (addr_of_mvector r + j)
+    \<Longrightarrow> (\<And>x. x \<noteq> addr_of_mvector r + j \<Longrightarrow> f x = g x) \<Longrightarrow> (\<And>z. f z = g z)"
     by smt
-  hence "\<And>z. (\<lambda>i. if i = addr_of_mvector r + Addr j then to_nat x else memory (h\<lparr>memory := \<lambda>i. if i = addr_of_mvector r + Addr j then to_nat y else memory h i\<rparr>) i) z
-    = (\<lambda>i. if i = addr_of_mvector r + Addr j then to_nat x else memory h i) z"
+  hence "\<And>z. (\<lambda>i. if i = addr_of_mvector r + j then to_nat x else memory (h\<lparr>memory := \<lambda>i. if i = addr_of_mvector r + j then to_nat y else memory h i\<rparr>) i) z
+    = (\<lambda>i. if i = addr_of_mvector r + j then to_nat x else memory h i) z"
     by auto
-  thus "h\<lparr>memory := \<lambda>i. if i = addr_of_mvector r + Addr j then to_nat x else memory (h\<lparr>memory := \<lambda>i. if i = addr_of_mvector r + Addr j then to_nat y else memory h i\<rparr>) i\<rparr>
-    = h\<lparr>memory := \<lambda>i. if i = addr_of_mvector r + Addr j then to_nat x else memory h i\<rparr>"
+  thus "h\<lparr>memory := \<lambda>i. if i = addr_of_mvector r + j then to_nat x else memory (h\<lparr>memory := \<lambda>i. if i = addr_of_mvector r + j then to_nat y else memory h i\<rparr>) i\<rparr>
+    = h\<lparr>memory := \<lambda>i. if i = addr_of_mvector r + j then to_nat x else memory h i\<rparr>"
     by simp
 qed
 
@@ -67,6 +71,87 @@ lemma execute_read: "execute (read v i) h = (get_at h v i, h)"
 
 lemma execute_writ: "execute (writ r i v) h = ((), set_at r i v h)"
   by (simp add: writ_def)
+
+lemma effect_read:
+  assumes "effect (read arr i) h h' r"
+  shows "r = get_at h arr i" "h = h'"
+  apply (metis assms effectE execute_read prod.sel(1))
+  apply (metis assms effectE execute_tap read_def snd_conv)
+  done
+
+lemma effect_writ:
+  assumes "effect (writ arr i v) h h' ()"
+  shows "h' = set_at arr i v h"
+  by (metis (full_types) assms effectE execute_writ snd_conv)
+
+lemma effect_swap:
+  assumes "effect (swap arr i j) h h' ()"
+  and "i \<noteq> j"
+  shows "get_at h arr i = get_at h' arr j" and "get_at h arr j = get_at h' arr i"
+proof-
+  obtain h1 ri rj where
+    "effect (read arr i) h h ri"
+    "effect (read arr j) h h rj"
+    "effect (writ arr j ri) h h1 ()"
+    "effect (writ arr i rj) h1 h' ()"
+  proof-
+    have "effect (do {
+      ri \<leftarrow> read arr i;
+      rj \<leftarrow> read arr j;
+      writ arr j ri;
+      writ arr i rj;
+      return ()
+    }) h h' ()"
+      using assms
+      by (simp add: swap_def)
+    then obtain ri where
+      e1: "effect (read arr i) h h ri"
+      "effect (do {
+        rj \<leftarrow> read arr j;
+        writ arr j ri;
+        writ arr i rj;
+        return ()
+      }) h h' ()"
+      by (metis (no_types, lifting) effect_bind effect_read(2))
+    then obtain rj where
+      e2: "effect (read arr j) h h rj"
+      "effect (do {
+        writ arr j ri;
+        writ arr i rj;
+        return ()
+      }) h h' ()"
+      by (metis (no_types, lifting) effect_bind effect_read(2))
+    then obtain h1 where
+      e3: "effect (writ arr j ri) h h1 ()"
+      "effect (do { writ arr i rj; return () }) h1 h' ()"
+      using effect_bind by force
+    hence e4: "effect (writ arr i rj) h1 h' ()"
+      by simp
+
+    assume H: "(\<And>ri rj h1. effect (read arr i) h h ri \<Longrightarrow> effect (read arr j) h h rj \<Longrightarrow> effect (writ arr j ri) h h1 () \<Longrightarrow> effect (writ arr i rj) h1 h' () \<Longrightarrow> thesis)"
+    show ?thesis
+      apply (rule H)
+      apply (rule e1)
+      apply (rule e2)
+      apply (rule e3)
+      apply (rule e4)
+      done
+  qed
+
+  have "ri = get_at h arr i"
+    using \<open>effect (read arr i) h h ri\<close> effect_read(1) by blast
+  have "rj = get_at h arr j"
+    using \<open>effect (read arr j) h h rj\<close> effect_read(1) by blast
+  have h': "h' = set_at arr i rj (set_at arr j ri h)"
+    using \<open>effect (writ arr i rj) h1 h' ()\<close> \<open>effect (writ arr j ri) h h1 ()\<close> effect_writ by blast
+
+  show "get_at h arr i = get_at h' arr j"
+    apply (simp add: h')
+    sorry
+  show "get_at h arr j = get_at h' arr i"
+    sorry
+qed
+
 
 (*
 fast implementation
@@ -86,7 +171,7 @@ definition to_list :: "'a::heap mvector \<Rightarrow> 'a list io" where
   "to_list vec = (let s = size_of_mvector vec in mapM (read vec) [0..<s])"
 
 definition set_over :: "'a::heap mvector \<Rightarrow> 'a::heap list \<Rightarrow> heap \<Rightarrow> heap" where
-  "set_over r xs h = h \<lparr> memory := (\<lambda>i. if lim h < i \<and> i < lim h + Addr (size xs) then to_nat (get_at h r (nat_of_addr (i - lim h))) else memory h i) \<rparr>"
+  "set_over r xs h = h \<lparr> memory := (\<lambda>i. if lim h < i \<and> i < lim h + size xs then to_nat (get_at h r (i - lim h)) else memory h i) \<rparr>"
 
 lemma execute_from_list: "execute (from_list xs) h = (case alloc (size xs) h of (mvec,h0) \<Rightarrow> (mvec, fold (\<lambda>(i,x) h. set_at mvec i x h) (enumerate 0 xs) h0))"
 proof-
